\documentclass{article}
\title{HW 2}
\usepackage[utf8]{inputenc}
\usepackage{hyperref} % for hyperlinks
\usepackage{amssymb}
\usepackage{authblk}
\usepackage{minted}   % for code linting
\usepackage{amsmath}   % big brackets
\author{Joshua Ortiga \\
		\and
		Xin Li \\
		\and
		Jonathan Le}
\begin{document}

\maketitle
\textbf{Problem 2.1.} Define the following sets $S_n \subset \mathbb{R}$

\begin{center}
	$S_n = \{x|x \in \mathbb{R}, 0 < x < \frac{1}{n}\}$.
\end{center}

\hspace{1cm} Define the following set:

\begin{center}
	$S = \displaystyle\bigcap_{n=1}^{\infty} S_n = S_1 \cap S_2 \cap S_3 \cap ....$
\end{center}

\hspace{1cm} Prove that $S = $ \o.

\vspace{0.5cm}

\textbf{Problem 2.2.} Let $F_n$ be the $n\textsuperscript{th}$ Fibonacci number. Prove that $\forall n \in \mathbb{N}$, 

$gcd(F_n,F_n+1) = 1$.

\vspace{0.3cm}

In the Fibonacci sequence: $F_n+1 = F_n + F_n-1$.

\vspace{0.2cm}

$\therefore gcd(F_n + F_n-1, F_n) = gcd(F_n+1, F_n)$.

\vspace{0.2cm}

Base case: $gcd(F_1, F_2) = 1$, \hspace{0.2cm} $(F_1 = 1, F_2 = 1)$

\vspace{0.2cm}

Assume that: $(F_n-1, F_n) = 1$, \hspace{0.2cm} where $n \geq 2$.

\vspace{0.2cm}

Since: $F_n+1 = F_n + F_n-1$, and $gcd(F_n + F_n-1, F_n) = gcd(F_n, F_n+1)$

\vspace{0.2cm}

$\therefore gcd(F_n, F_n+1) = 1 \hspace{0.5cm} \blacksquare$

\vspace{0.5cm}

\textbf{Problem 2.3.} $\forall n \in \mathbb{N}$, prove that

\begin{center}
	$\displaystyle\sum_{k=1}^{n} k^3 = \left(\displaystyle\sum_{k=1}^{n} k\right)^2$.
\end{center}

Assume that: $\displaystyle\sum_{k=1}^{n} k = \frac{n(n+1)}{2}$.

Then: 	$\left(\displaystyle\sum_{k=1}^{n} k \right)^2 =  \left(\frac{n(n+1)}{2}\right)^2 = \frac{n^2(n+1)^2}{4}$.

Now then, assume that: $\displaystyle\sum_{k=1}^{n} k^3 = \frac{n^2(n+1)^2}{4}$.

Inductive step: Assume $\left(\frac{n(n+1)}{2}\right)^2$ to be true $\forall n$ up until $(n+1)$. 

Use $P(n) \Rightarrow P(n+1)$.

\vspace{0.5cm}

$P(n+1) = \left(\frac{n(n+1)}{2} + (n+1) \right)^2$

\vspace{0.2cm}
\hspace{2cm} $\downarrow$
\vspace{0.2cm}


$\left(\frac{n^2+n}{2} + (n+1)\right)^2 = \left(\frac{n^2+3n+2}{2}\right)^2$

\vspace{0.5cm}

$= \frac{(n^2+3n+2)(n^2+3n+2)}{4} = \frac{n^4+3n^3+2n^2+3n^3+9n^2+6n+2n^2+6n+4}{4}$

\vspace{0.5cm}

$= \frac{n^4+6n^3+13n^2+12n+4}{4} = \frac{(n+1)(n+1)(n+2)(n+2)}{4} = \frac{(n+1)^2(n+2)^2}{4}$

\vspace{1.2cm}

$P(n+1)$ for $\displaystyle\sum_{k=1}^{n} k^3 = \frac{n^2(n+1)^2}{4} + (n+1)^3$

$= \frac{n^2(n^2+2n+1)}{4} + \frac{4(n+1)^3}{4} = \frac{n^4+2n^3+n^2}{4} + \frac{4(n^3+3n^2+3n+1)}{4}$

\vspace{0.3cm}

$= \frac{n^4+2n^3+n^2+4n^3+12n^2+12n+4}{4} = \frac{n^4+6n^3+13n^2+12n+4}{4}$

\vspace{0.3cm}

$= \frac{(n+1)(n+1)(n+2)(n+2)}{4} = \frac{(n+1)^2(n+2)^2}{4}$

\vspace{0.3cm}

$\therefore $ Since $ \left(\frac{n(n+1)}{2} + (n+1) \right)^2 = \frac{n^2(n+1)^2}{4} + (n+1)^3 $ 

$\displaystyle\sum_{k=1}^{n} k^3 = \left( \displaystyle\sum_{k=1}^{n} k \right)^2 \blacksquare $

\vspace{3.2cm}

\textbf{Problem 2.4.} Prove that for a list of any size, the function below will 

return the largest item from the list.

\vspace{0.5cm}

\hrule

\begin{minted}{python}
    if len(lst) == 0:
        return None
    elif len(lst) == 1:
        return lst[0]
    # lst[~0] represents the last item in the array
    # equivilent to lst[-1]
    maximum = maxItem(lst[:~0])
    if lst[~0] < maximum:
        return maximum
    else:
        return lst[~0]
\end{minted}

\hrule

\vspace{0.5cm}

Let the list $foo$ = [4, 3, 2, 5, 1, 6, 2].

\vspace{0.5cm}

Following the code given: $foo$ is broken up into pairs comparing each 

value with the next element, starting from index 0, and returning the largest 

value in each pair through every recursive iteration.

\vspace{0.5cm}

\underline{Function calls}

1. $maximum = maxItem([4,3,2,5,1,6])$

2. $maximum = maxItem([4,3,2,5,1])$

3. $maximum = maxItem([4,3,2,5])$

4. $maximum = maxItem([4,3,2])$

5. $maximum = maxItem([4,3])$

6. $maximum = maxItem([4])$ $\leftarrow$ Base case reached, len($foo$) = 1

\vspace{0.5cm}

\underline{Returning}


1. $maximum = 4$

2. $maximum = 4$ $(3 < 4)$ $\leftarrow$ pair

3. $maximum = 4$ $(2 < 4)$ $\leftarrow$ pair

4. $maximum = 5$ $(5 \not < 4)$ $\leftarrow$ pair

5. $maximum = 5$ $(1 < 5)$ $\leftarrow$ pair

6. $maximum = 6$ $(6 \not < 5)$  $\leftarrow$ pair

\vspace{0.5cm}

6 is the largest item in $foo$.

\vspace{0.2cm}

$\therefore$ Since $foo[$\textasciitilde{}$0] < maximum$ will always check for the larger value in each 

pair, and return it if $foo[$\textasciitilde{}$0]$ is not more than the current largest value in 

the list (or else, $foo[$\textasciitilde{}$0]$ would be returned as the new current maximum 

value), the function will always return the largest item from the list of any 

size. \hspace{0.5cm} $\blacksquare$


\end{document}

